src/Lean/Meta/Tactic/Cbv.lean
@@ -16,48 +16,91 @@ structure EvalResult where
 def mkRefl (e : Expr) : MetaM EvalResult := do
   return {value := e, proof := (← mkEqRefl e) }
 
-mutual
- partial def evalCbv (e : Expr) : MetaM EvalResult := do
+def isValue (e : Expr) : MetaM Bool := do
   match e with
-  | .lam _ _ _ _ => return {value := e, proof := (← mkEqRefl e) }
+  | .lam _ _ _ _ => return false
+  | .const name _ =>
+    let info ← getConstInfo name
+    return info.isCtor
   | .app fn arg =>
-      evalApp fn arg
-  | _ => mkRefl e
-
-
-  partial def evalApp (f arg : Expr) : MetaM EvalResult := do
-    let ⟨fRes, fProof⟩ ← evalCbv f
-    trace[Meta.Tactic] "Lhs: {f} -*-> {fRes}"
-    let ⟨argRes, argProof⟩ ← evalCbv arg
-    trace[Meta.Tactic] "Rhs: {arg} -*-> {argRes}"
-    if fRes.isLambda then
-      trace[Meta.Tactic] "{fRes} is a lambda expression"
-      return {value := .app f arg, proof := (← mkEqRefl (.app f arg)) }
+    if (← isValue fn) then
+      isValue arg
     else
-      trace[Meta.Tactic] "{fRes} is a function application"
+      return false
+  | .forallE _ _ _ _ => return false
+  | .lit _ => return true
+  | .proj _ _ _ => return false
+  | .mdata _ e => isValue e
+  | .bvar _ => return false
+  | .letE _ _ _ _ _ => return false
+  | .sort _ => return true
+  | .mvar _ => return false
+  | .fvar _  => return false
+
+mutual
+ partial def evalCbv (e : Expr) (fuel : Nat) : MetaM EvalResult := do
+  trace[Meta.Tactic] "Fuel is: {fuel}"
+  if (fuel = 0) then
+    throwError "ran out of fuel"
+  let isVal ← isValue e
+  if isVal then
+    trace[Meta.Tactic] "Returning, as detected a value {e}"
+    mkRefl e
+  else
+    match e with
+    | .lam _ _ _ _ => mkRefl e
+    | .app fn arg =>
+        evalApp fn arg (fuel - 1)
+    | .letE _ _ _ _ _ => evalCbv (← zetaReduce e) (fuel-1)
+    | .proj _ _ _ =>
+      let some reduced ← reduceProj? e | throwError "could not reduce projection"
+      evalCbv (reduced) (fuel-1)
+
+    | _ => mkRefl e
+
+  partial def evalApp (f arg : Expr) (fuel : Nat) : MetaM EvalResult := do
+    trace[Meta.Tactic] "fuel {fuel}, evaluating {f} with argument {arg}"
+    let ⟨fRes, fProof⟩ ← evalCbv f (fuel - 1)
+    let ⟨argRes, argProof⟩ ← evalCbv arg (fuel - 1)
+    trace[Meta.Tactic] "lhs : {f} -*-> {fRes}, {arg} -*-> {argRes}"
+    if fRes.isLambda then
+      evalCbv (← instantiateLambda f #[arg]) (fuel - 1)
+    else
       let appFn := fRes.getAppFn.constName
-      trace[Meta.Tactic] "We got: {appFn}"
-      try
+      let info ← getConstInfo appFn
+      trace[Elab.Meta] "info for Fn: {info.isCtor}"
+      match info with
+      | .axiomInfo _ => throwError "not Supported axiom"
+      | .thmInfo _   => throwError "not Supported thm"
+      | .opaqueInfo _  => throwError "not Supported opaque"
+      | .quotInfo _ => throwError "not Supported quot"
+      | .inductInfo _ => throwError "not Supported induct"
+      | .ctorInfo _ =>
+          let ⟨bodyRes, bodyProof⟩ ← evalCbv arg (fuel - 1)
+
+          let resProof ← mkCongrArg f bodyProof
+          return {value := mkApp f bodyRes, proof := resProof}
+
+      | .recInfo _ => throwError "not Supported rec"
+      | .defnInfo info   =>
         let unfoldRes ← unfold (.app f arg) appFn
         let fallback ← mkEqRefl (.app f arg)
-        let proof := Option.getD (unfoldRes.proof?) fallback
+        let some proof := unfoldRes.proof? | throwError "Couldnt unfold"
         let resExpr := unfoldRes.expr
-        trace[Meta.Tactic] "res: {resExpr}"
+        if resExpr == (.app f arg) then
+          throwError "Didnt unfold"
+        trace[Meta.Tactic] "resExpr: {resExpr}"
+        let ⟨finalRes, finalProof⟩ ← evalCbv resExpr (fuel - 1)
+        let lhs ← mkCongr fProof argProof
+        let final ← mkEqTrans (← mkEqTrans lhs proof) finalProof
+        return {value := finalRes, proof := final}
 
-
-
-      catch _ =>
-        trace[Meta.Tactic] "Didnt succeed unfolding"
-
-
-
-      return {value := .app f arg, proof := (← mkEqRefl (.app f arg)) }
 end
 
 def cbv (e : Expr) : MetaM EvalResult := do
   trace[Meta.Tactic] "Trying to evaluate expression {e}"
 
-  evalCbv e
+  evalCbv e 100
 
 
 end Lean.Meta
